changing the semantics of QMOd so it doesn't require that q \sigma is not empty

QSemantics.thy
@@ -1,111 +1,63 @@
 (* Title:     Quantum-Semantics/QSemantics.thy
-   Author:    David Sanan, Nanyang Technological University 
-   Copyright   2020
+   Author:    David Sanan, Singapore Institute of Technology 
+   Copyright   2023
    License:     BSD
 *)
 
 theory QSemantics
-  imports QSyntax vars 
+  imports QSemanticsBig
 begin
 
 subsection \<open>Syntax\<close>
 
 text \<open>Semantics for quantum programs\<close>
 
-primrec redex:: "('a,'b,'s) com \<Rightarrow> ('a,'b,'s) com"
+primrec redex:: "('a,'s) com \<Rightarrow> ('a,'s) com"
 where
 "redex Skip = Skip" |
 "redex (SMod f) = (SMod f)" |
-"redex (QMod m e) = (QMod m e)" |
+"redex (QMod m q) = (QMod m q)" |
 "redex (Seq c\<^sub>1 c\<^sub>2) = redex c\<^sub>1" |
 "redex (IF b c\<^sub>1 c\<^sub>2) = (IF b c\<^sub>1 c\<^sub>2)" |
 "redex (While b c) = (While b c)" |
 "redex (Measure v q) = Measure v q" |
-"redex (Alloc v e l) = Alloc v e l" |
-"redex (Dispose e) = Dispose e"
-
+"redex (Alloc var v) = Alloc var v " |
+"redex (Dispose v q) = Dispose v q"
 
 
 (* m = partial_state2.ptensor_mat (dims_heap \<vv>) (q \<sigma>) ((Q_domain \<vv>)-(q \<sigma>)) (M::complex mat) (1\<^sub>m (card ((Q_domain \<vv>) - (q \<sigma>))))*)
 (* abbreviation "tensor_vec \<equiv> partial_state2.ptensor_vec" *)
 
+(* definition
+  unit_vecl :: "nat \<Rightarrow> nat \<Rightarrow> complex list"
+  where "unit_vecl n i = list_of_vec (unit_vec n i)" *)
 
-definition matrix_sep :: "nat set \<Rightarrow> (complex) QState \<Rightarrow> complex mat \<Rightarrow> complex vec" 
-  where "matrix_sep sep_vars qs M \<equiv>
-           let var_d = QState_vars qs in 
-           let var_r = var_d - sep_vars in
-           let v = QState_vector qs in           
-           let m = partial_state2.ptensor_mat sep_vars var_r
-                                        (M::complex mat) (1\<^sub>m (2^(card var_r)))  in           
-               (m *\<^sub>v v)
-        "
 
-(* definition alloc_vars :: "'q::linorder set \<Rightarrow> ('q, complex) QState \<Rightarrow> complex vec \<Rightarrow> complex vec"
-  where "alloc_vars sep_vars qs v \<equiv>            
-           partial_state2.ptensor_vec (list_dims (QState_vars qs)@list_dims sep_vars)
-                  (lin_set (QState_vars qs)) (lin_sets (top_lin_set ((QState_vars qs))) sep_vars)
-                  ( QState_vector qs) v" *)
-
-(* definition dispose_vars:: " 'q::linorder set \<Rightarrow> ('q, complex) QState \<Rightarrow> complex vec set"
-  where "dispose_vars sep_vars qs \<equiv> 
-   let vars_dom = QState_vars qs in
-   let v =   QState_vector qs in
-   let qv = (sorted_list_of_set vars_dom) in
-   let t = sorted_list_of_set sep_vars in
-   let l =  sorted_list_of_set (vars_dom - sep_vars) in
-   let qv' = t @ l in
-   let qn =  v.\<^sub>qv \<^sub>\<leadsto> \<^sub>qv' in 
-   let vars_dom' = vars_dom \<union> sep_vars in
-    {q. (\<exists>q2. qn = partial_state.tensor_vec (list_dims vars_dom) {0..<card sep_vars} q q2)}" *)
-
-(* definition measure_vars::"nat \<Rightarrow>  nat set \<Rightarrow> (complex) QState  \<Rightarrow> (real\<times>complex vec)"
-  where "measure_vars k  sep_vars qs \<equiv>
-   let vars_dom = QState_vars qs in
-    let v =   QState_vector qs in
-    let vars= (vars_dom - sep_vars) in
-    let l = (sorted_list_of_set sep_vars) in
-    let t = (sorted_list_of_set vars) in
-    let qv = (sorted_list_of_set vars_dom) in
-    let qv' = l @ t in 
-    let qn = v.\<^sub>qv \<^sub>\<leadsto> \<^sub>qv'  in
-    let mk = partial_state2.ptensor_mat  vars_dom vars (1\<^sub>k (2^(length l))) (1\<^sub>m (2^(length t))) in
-    let qn' =  mk  *\<^sub>v v in 
-    let \<delta>k =  Re (((mat_adjoint (mat_of_rows (dim_vec v) [v]) *\<^sub>v qn') $ 0) div vec_norm qn') in    
-    let qnprod = ((sqrt \<delta>k)::complex) \<cdot>\<^sub>v qn' in
-       (\<delta>k, qnprod.\<^sub>qv' \<^sub>\<leadsto> \<^sub>qv)" *)
-
-definition measure_vars::"nat \<Rightarrow>  nat set \<Rightarrow> (complex) QState  \<Rightarrow> (real\<times>complex vec)"
-  where "measure_vars k  sep_vars qs \<equiv>
-   let vars_dom = QState_vars qs in
-    let v =   QState_vector qs in
-    let vars= (vars_dom - sep_vars) in    
-    let mk = partial_state2.ptensor_mat  vars_dom vars (1\<^sub>k (2^(card vars_dom))) (1\<^sub>m (2^(card vars))) in
-    let qn' =  mk  *\<^sub>v v in 
-    let \<delta>k =  Re (((mat_adjoint (mat_of_rows (dim_vec v) [v]) *\<^sub>v qn') $ 0) div vec_norm qn') in    
-    let qnprod = ((sqrt \<delta>k)::complex) \<cdot>\<^sub>v qn' in
-       (\<delta>k, qnprod)" 
 
 context vars
 begin
 
-inductive QStep::"('v,'b,'s) QConf \<Rightarrow> ('v,'b,'s) QConf \<Rightarrow> bool" 
+inductive step::"('v,'s) QConf \<Rightarrow> ('v,'s) QConf \<Rightarrow> bool" 
   ("\<turnstile> _ \<rightarrow> _" [81,81] 80)  
   where 
-  Skip : "\<turnstile> (Skip, Normal \<sigma>) \<rightarrow> (Skip, Normal \<sigma>)" 
 \<comment>\<open>SMod  modifies the stack of non-qubits variables \<sigma> with f \<sigma>, where f is a 
   function modifying the stack\<close>
- | StackMod: "\<turnstile> (SMod f, Normal (\<delta>,\<sigma>,\<Q>)) \<rightarrow> (Skip, Normal (\<delta>,f \<sigma>,\<Q>))"
+  StackMod: "\<turnstile> (SMod f, Normal (\<delta>,\<sigma>,\<Q>)) \<rightarrow> (Skip, Normal (\<delta>,f \<sigma>,\<Q>))"
 
 \<comment>\<open>QMod modifies the set of qubits of the Quantum State given by q \<sigma> with the 
   transformation matrix M, any qubit not included in q \<sigma> remains the same\<close>
 
- | QMod:"(q \<sigma>)\<noteq>{} \<Longrightarrow> (q \<sigma>) \<subseteq> (QState_vars \<qq>) \<Longrightarrow> 
-         \<qq>' = matrix_sep (q \<sigma>) \<qq> m \<Longrightarrow>
-         \<turnstile> (QMod M q, Normal (\<delta>,\<sigma>,(\<vv>,\<qq>))) \<rightarrow> (Skip, Normal (\<delta>, \<sigma>,(\<vv>,QState(QState_vars \<qq>, list_of_vec  \<qq>'))))"
+ | QMod:"\<forall>e \<in> (q \<sigma>). (QStateM_map \<Q>) e \<noteq> {}  \<Longrightarrow> unitary M \<Longrightarrow>
+         \<Q>' = matrix_sep_QStateM (q \<sigma>) \<Q> M \<Longrightarrow>  
+         M \<in> carrier_mat (2 ^ card (\<Union> (QStateM_map \<Q> ` (q \<sigma>))))  
+                         (2 ^ card (\<Union> (QStateM_map \<Q> ` (q \<sigma>)))) \<Longrightarrow>      
+         \<turnstile> (QMod M q, Normal (\<delta>,\<sigma>, \<Q>)) \<rightarrow> (Skip,Normal (\<delta>, \<sigma>,  \<Q>'))"
 
 \<comment>\<open>QMod fails if the set of qubits to be modified is not included in the quantum state\<close>
- | QMod_F:"\<not> ((q \<sigma>) \<subseteq> (QState_vars \<qq>)) \<Longrightarrow>          
-          \<turnstile> (QMod M q, Normal (\<delta>,\<sigma>,(\<vv>,\<qq>))) \<rightarrow> (Skip, Fault)"
+ | QMod_F:"\<exists>e. e \<in> q \<sigma> \<and> (QStateM_map \<Q>) e = {}  \<or>  \<not> unitary M  \<or> 
+         M \<notin> carrier_mat (2 ^ card (\<Union> (QStateM_map \<Q> ` (q \<sigma>))))  
+                         (2 ^ card (\<Union> (QStateM_map \<Q> ` (q \<sigma>))))  \<Longrightarrow>        
+          \<turnstile> (QMod M q, Normal (\<delta>,\<sigma>, \<Q>)) \<rightarrow> (Skip, Fault)"
 
 \<comment>\<open>Alloc takes a normal variable "q" representing the variable where the index to the qubits is store
    an function e from the state \<sigma> to a natural number representing the number of qubits to allocate
@@ -115,15 +67,15 @@ inductive QStep::"('v,'b,'s) QConf \<Rightarrow> ('v,'b,'s) QConf \<Rightarrow> 
   We will require that a program is well formed, meaning that the types are correct.
   A call to Alloc is well formed if the ty"'s state"pe of q is a natural number\<close>
 
- | Alloc:"q' \<notin> (dom_q_vars \<vv>) \<Longrightarrow> q'_addr \<in> new_q_addr (e \<sigma>) \<vv> \<Longrightarrow>
-          \<vv>' = \<vv>(q' := q'_addr)  \<Longrightarrow> length (v \<sigma>) = (e \<sigma>) \<Longrightarrow> \<sigma>' = set_value \<sigma> q (nat_to_typ q') \<Longrightarrow>                    
-          \<turnstile> (Alloc q e v, Normal (\<delta>,\<sigma>,(\<vv>,\<qq>))) \<rightarrow> (Skip, Normal (\<delta>, \<sigma>',(\<vv>',\<qq> + QState (q'_addr,(v \<sigma>)) )))"
-
+ | Alloc:"q' \<notin> (dom_q_vars (QStateM_map \<Q>)) \<Longrightarrow> (length (v \<sigma>) > 1) \<Longrightarrow> 
+              \<vv>' = (\<lambda>i. {})(q' := q'_addr) \<and>  \<sigma>' = set_value \<sigma> q (from_nat q') \<Longrightarrow> 
+          q'_addr \<in> new_q_addr v \<sigma> (QStateM_map \<Q>)  \<Longrightarrow> vec_norm (vec_of_list (v \<sigma>)) = 1 \<Longrightarrow>
+          \<turnstile> (Alloc q v, Normal (\<delta>,\<sigma>, \<Q>))\<rightarrow> (Skip, Normal (\<delta>, \<sigma>', \<Q> + Q_State.QStateM(\<vv>', QState (q'_addr,(v \<sigma>)) )))"
 \<comment>\<open>Alloc will fail if the length of the initial value is not equal to the number of qubits allocated \<close>
 
 
- | Alloc_F:"length (v \<sigma>) \<noteq> (e \<sigma>) \<Longrightarrow>                    
-          \<turnstile> (Alloc q e v, Normal (\<delta>,\<sigma>,(\<vv>,\<qq>))) \<rightarrow> (Skip, Fault)"
+ | Alloc_F:"length (v \<sigma>) \<le> 1 \<or>  vec_norm (vec_of_list (v \<sigma>)) \<noteq> 1 \<Longrightarrow>                    
+          \<turnstile> (Alloc q v, Normal (\<delta>,\<sigma>,\<Q>)) \<rightarrow> (Skip, Fault)"
 
 \<comment>\<open>the conditional, while, and seq statements follow the standard definitions\<close>
 
@@ -137,7 +89,7 @@ inductive QStep::"('v,'b,'s) QConf \<Rightarrow> ('v,'b,'s) QConf \<Rightarrow> 
  | WhileFalse: "\<sigma>\<notin>b \<Longrightarrow> 
                  \<turnstile> (While b c, Normal (\<delta>,\<sigma>,\<Q>)) \<rightarrow> (Skip, Normal (\<delta>,\<sigma>,\<Q>))"
 
- | Seq:"\<lbrakk>\<turnstile> (C1, \<sigma>) \<rightarrow> (C1', \<sigma>')\<rbrakk> \<Longrightarrow> \<turnstile> (Seq C1 C2, \<sigma>) \<rightarrow> (C1'C2, \<sigma>')"
+ | Seq:"\<lbrakk>\<turnstile> (C1, \<sigma>) \<rightarrow> (C1', \<sigma>')\<rbrakk> \<Longrightarrow> \<turnstile> (Seq C1 C2, \<sigma>) \<rightarrow> (Seq C1' C2, \<sigma>')"
 
 | SeqSkip: "\<turnstile> (Seq Skip C2,\<sigma>) \<rightarrow> (C2, \<sigma>)"
 
@@ -146,40 +98,430 @@ inductive QStep::"('v,'b,'s) QConf \<Rightarrow> ('v,'b,'s) QConf \<Rightarrow> 
   Quantum state. The entanglement condition is that it is possible to find a vector \<qq>1 such that
   \<qq> =  \<qq>' +  \<qq>''\<close>
 
- | Dispose: "\<vv> (q \<sigma>) \<noteq> {} \<Longrightarrow> \<vv>' = \<vv>((q \<sigma>):={}) \<Longrightarrow> \<qq>' ## \<qq>''  \<Longrightarrow> 
-            \<vv> (q \<sigma>) = QState_vars \<qq>'' \<Longrightarrow> \<qq> =   \<qq>' +  \<qq>'' \<Longrightarrow>            
-             \<turnstile> (Dispose q, Normal (\<delta>,\<sigma>,(\<vv>,\<qq>))) \<rightarrow> (Skip,Normal (\<delta>,\<sigma>,(\<vv>',\<qq>')))"
-
+| Dispose: "  \<Q>' ## \<Q>'' \<Longrightarrow> \<Q> =  \<Q>' + \<Q>'' \<Longrightarrow> 
+              QStateM_vars \<Q>' \<noteq> {} \<Longrightarrow> Zero \<Q>' \<Longrightarrow>
+              QStateM_vars \<Q>' = (Q_domain_var (the (var_set q i \<sigma>)) (QStateM_map \<Q>')) \<Longrightarrow>                                      
+              \<forall>e \<in> (the (var_set q i \<sigma>)). (QStateM_map \<Q>') e \<noteq> {} \<Longrightarrow>
+             \<turnstile> (Dispose q i, Normal (\<delta>,\<sigma>,\<Q>)) \<rightarrow> (Skip, Normal (\<delta>,\<sigma>,  \<Q>''))"
 \<comment>\<open>Dispose dispose will fail if it is not possible to find such states \<qq>',  \<qq>''\<close>
 
 
- | Dispose_F: "\<nexists>\<qq>' \<qq>''. \<vv> (q \<sigma>) \<noteq> {} \<and> \<vv> (q \<sigma>) = QState_vars \<qq>'' \<and> 
-               \<qq> =   \<qq>' +  \<qq>'' \<and> \<qq>' ## \<qq>'' \<Longrightarrow>
-               \<turnstile> (Dispose q, Normal (\<delta>,\<sigma>,(\<vv>,\<qq>))) \<rightarrow> (Skip,Fault)"
+ | Dispose_F:  "(\<nexists>\<Q>' \<Q>''.  \<Q> = \<Q>' + \<Q>'' \<and> \<Q>' ## \<Q>'' \<and> QStateM_vars \<Q>' \<noteq> {} \<and> Zero \<Q>' \<and> 
+               QStateM_vars \<Q>' = (Q_domain_var (the (var_set q i \<sigma>)) (QStateM_map \<Q>')) \<and>
+               (\<forall>e \<in> (the (var_set q i \<sigma>)). (QStateM_map \<Q>') e \<noteq> {})) \<Longrightarrow>
+               \<turnstile> (Dispose q i, Normal (\<delta>,\<sigma>,\<Q>)) \<rightarrow> (Skip, Fault)"
 
 \<comment>\<open>Measure measures the value of the set of qubits given by q \<sigma> and it stores the result in 
   the stack variable v. Similar to allocate, we will require that the construct is well formed
  and that the type of v is a real number\<close>
 
- | Measure: "q \<sigma> \<subseteq> (QState_vars \<qq>) \<Longrightarrow> 
-            (\<delta>k, \<qq>') = measure_vars k (q \<sigma>) \<qq> \<Longrightarrow>
-            \<delta>k > 0 \<Longrightarrow> \<delta>' = \<delta> * \<delta>k \<Longrightarrow> 
-            \<turnstile> (Measure v q, Normal (\<delta>,\<sigma>,(\<vv>,\<qq>))) \<rightarrow> (Skip,Normal (\<delta>',\<sigma>,(\<vv>,QState(Q_domain \<vv>', list_of_vec  \<qq>'))))" 
-
+ | Measure: "addr1 = \<Union>((QStateM_map \<Q>) ` (q \<sigma>)) \<Longrightarrow> \<forall>e \<in> (q \<sigma>). (QStateM_map \<Q>) e \<noteq> {} \<Longrightarrow>                      
+            k \<in> {0..<2^(card addr1)} \<Longrightarrow>          
+            (\<delta>k, \<Q>') = measure_vars k (q \<sigma>) \<Q> \<Longrightarrow>             
+            \<delta>k > 0 \<Longrightarrow> \<delta>' = \<delta> * \<delta>k \<Longrightarrow> \<sigma>' = set_value \<sigma> v (from_nat k) \<Longrightarrow>
+            \<turnstile> (Measure v q, Normal (\<delta>,\<sigma>,\<Q>)) \<rightarrow> (Skip, Normal (\<delta>',\<sigma>', \<Q>'))"
 \<comment>\<open>Since Measure access to the values of the qubits given by q \<sigma> as QMod, 
   Measure will similarly fail if the set of qubits to be mesured does not
   belong to the set of allocated qubits\<close>
 
- | Measure_F: "\<not> (q \<sigma> \<subseteq> (QState_vars \<qq>)) \<Longrightarrow>  
-              \<turnstile> (Measure v q, Normal (\<delta>,\<sigma>,(\<vv>,\<qq>))) \<rightarrow> (Skip, Fault)" 
+ | Measure_F: "\<exists>e. e \<in> q \<sigma> \<and> (QStateM_map \<Q>) e = {}  \<Longrightarrow> 
+              \<turnstile> (Measure v q, Normal (\<delta>,\<sigma>,\<Q>)) \<rightarrow> (Skip, Fault)" 
 
-| Fault_Prop:" C\<noteq>Skip \<Longrightarrow> \<turnstile> (C, Fault) \<rightarrow> (Skip, Fault)"
+| Fault_Prop:"\<lbrakk>c\<noteq>Skip; redex c = c\<rbrakk> \<Longrightarrow>  \<turnstile> (c, Fault) \<rightarrow> (Skip, Fault)"
 
+thm step.intros
 
-lemmas step_induct = QStep.induct [of "(c,s)" "(c',s')", split_format (complete), case_names
+thm Fault_Prop
+
+inductive_cases QStep_elim_cases [cases set]:
+ "\<turnstile>(c,Fault) \<rightarrow>  t"  
+  "\<turnstile>(Skip,s) \<rightarrow>  t"
+  "\<turnstile>(SMod f,s) \<rightarrow>  t"
+  "\<turnstile>(QMod m q,s) \<rightarrow>  t"
+  "\<turnstile>(Seq c1 c2,s) \<rightarrow> t"
+  "\<turnstile>(While b c,s) \<rightarrow>  t"
+  "\<turnstile>(IF b c1 c2,s) \<rightarrow>  t"
+  "\<turnstile>(Measure v q,s) \<rightarrow>  t"
+  "\<turnstile>(Alloc v  e,s) \<rightarrow>  t"
+  "\<turnstile>(Dispose q i,s) \<rightarrow>  t"
+
+inductive_cases QStep_Normal_elim_cases [cases set]:
+ "\<turnstile>(c,Fault) \<rightarrow>  t"  
+  "\<turnstile>(Skip,Normal s) \<rightarrow>  t"
+  "\<turnstile>(SMod f,Normal s) \<rightarrow>  t"
+  "\<turnstile>(QMod m q,Normal s) \<rightarrow>  t"
+  "\<turnstile>(Seq c1 c2,Normal s) \<rightarrow>  t"
+  "\<turnstile>(While b c1,Normal s) \<rightarrow>  t"
+  "\<turnstile>(IF b c1 c2,Normal s) \<rightarrow>  t"
+  "\<turnstile>(Measure v q,Normal s) \<rightarrow>  t"
+  "\<turnstile>(Alloc v  e,Normal s) \<rightarrow>  t"
+  "\<turnstile>(Dispose q v,Normal s) \<rightarrow>  t"
+
+inductive_cases QStep_Fault_elim_cases [cases set]:
+ "\<turnstile>(c,Fault) \<rightarrow>  (c',Fault)"  
+  "\<turnstile>(Skip,Normal s) \<rightarrow>  (c', Fault)"
+  "\<turnstile>(SMod f,Normal s) \<rightarrow>  (c', Fault)"
+  "\<turnstile>(QMod m q,Normal s) \<rightarrow> (c', Fault)"
+  "\<turnstile>(Seq c1 c2,Normal s) \<rightarrow> (c', Fault)"
+  "\<turnstile>(While b c1,Normal s) \<rightarrow> (c', Fault)"
+  "\<turnstile>(IF b c1 c2,Normal s) \<rightarrow>  (c', Fault)"
+  "\<turnstile>(Measure v q,Normal s) \<rightarrow>  (c', Fault)"
+  "\<turnstile>(Alloc v  e,Normal s) \<rightarrow>  (c', Fault)"
+  "\<turnstile>(Dispose q v,Normal s) \<rightarrow>  (c', Fault)"
+
+lemmas step_induct = step.induct [of "(c,s)" "(c',s')", split_format (complete), OF vars_axioms, case_names
 StackMod QMod QMod_F Alloc Alloc_F CondTrue CondFalse WhileTrue WhileFalse Seq SeqSkip Dispose
-Dispose Dispose_F Measure Measure_F Fault_Prop, induct set]
-end 
+Dispose_F Measure Measure_F Fault_Prop,induct set] 
+
+
+
+definition final:: "('v,'s) QConf \<Rightarrow> bool" where
+"final cfg \<equiv> (fst cfg=Skip)"
+
+abbreviation
+ "step_rtrancl" :: "[('v,'s) QConf,('v,'s) QConf] \<Rightarrow> bool"
+                                ("\<turnstile> (_ \<rightarrow>\<^sup>*/ _)" [81,81] 100)
+ where
+  "\<turnstile>cf0 \<rightarrow>\<^sup>* cf1 \<equiv> (CONST step)\<^sup>*\<^sup>* cf0 cf1"
+
+abbreviation
+ "step_trancl" :: "[('v,'s) QConf,('v,'s) QConf] \<Rightarrow> bool"
+                                ("\<turnstile> (_ \<rightarrow>\<^sup>+/ _)" [81,81] 100)
+ where
+  "\<turnstile>cf0 \<rightarrow>\<^sup>+ cf1 \<equiv> (CONST step)\<^sup>+\<^sup>+ cf0 cf1"
+
+
+lemma redex_not_Seq: "redex c = Seq c1 c2 \<Longrightarrow> P"
+  apply (induct c)
+  apply auto
+  done
+
+lemma no_step_final:
+  assumes step: "\<turnstile>(c,s) \<rightarrow> (c',s')"
+  shows "final (c,s) \<Longrightarrow> P"
+  using step
+  by (induct, auto simp add: final_def)
+
+thm no_step_final
+
+lemma no_step_final':
+  assumes step: "\<turnstile>cfg \<rightarrow> cfg'"
+  shows "final cfg \<Longrightarrow> P"
+using step by (cases cfg', cases cfg) (auto intro: no_step_final )
+
+
+lemma step_Fault': 
+  assumes step: "\<turnstile> (c,s) \<rightarrow>  (c',s')" and s1:"snd (c,s) = Fault"
+  shows "snd (c',s') = Fault"
+  using step s1 by (induct, auto)
+
+lemma step_Fault: 
+  assumes step: "\<turnstile> (c,s) \<rightarrow>  (c',s')"
+  shows "s = Fault \<Longrightarrow> s' = Fault"
+  using step_Fault'[OF step] by auto
+
+lemma SeqSteps:
+  assumes steps: "\<turnstile>cfg\<^sub>1\<rightarrow>\<^sup>* cfg\<^sub>2"
+  shows "\<And> c\<^sub>1 s c\<^sub>1' s'. \<lbrakk>cfg\<^sub>1 = (c\<^sub>1,s);cfg\<^sub>2=(c\<^sub>1',s')\<rbrakk>
+          \<Longrightarrow> \<turnstile>(Seq c\<^sub>1 c\<^sub>2,s) \<rightarrow>\<^sup>* (Seq c\<^sub>1' c\<^sub>2, s')"
+using steps
+proof (induct rule: converse_rtranclp_induct [case_names Refl Trans])
+  case Refl
+  thus ?case
+    by simp
+next
+  case (Trans cfg\<^sub>1 cfg'')
+  have step: "\<turnstile> cfg\<^sub>1 \<rightarrow> cfg''" by fact
+  have steps: "\<turnstile> cfg'' \<rightarrow>\<^sup>* cfg\<^sub>2" by fact
+  have cfg\<^sub>1: "cfg\<^sub>1 = (c\<^sub>1, s)" and cfg\<^sub>2: "cfg\<^sub>2 = (c\<^sub>1', s')"  by fact+
+  obtain c\<^sub>1'' s'' where cfg'': "cfg''=(c\<^sub>1'',s'')"
+    by (cases cfg'') auto
+  from step cfg\<^sub>1 cfg''
+  have "\<turnstile> (c\<^sub>1,s) \<rightarrow> (c\<^sub>1'',s'')"
+    by simp
+  hence "\<turnstile> (Seq c\<^sub>1 c\<^sub>2,s) \<rightarrow> (Seq c\<^sub>1'' c\<^sub>2,s'')"
+    by (rule step.Seq)
+  also from Trans.hyps (3) [OF cfg'' cfg\<^sub>2]
+  have "\<turnstile> (Seq c\<^sub>1'' c\<^sub>2, s'') \<rightarrow>\<^sup>* (Seq c\<^sub>1' c\<^sub>2, s')" .
+  finally show ?case .
+qed
+
+lemma steps_Fault: "\<turnstile> (c, Fault) \<rightarrow>\<^sup>* (Skip, Fault )"
+proof (induct c)
+  case (Seq c\<^sub>1 c\<^sub>2)
+  have steps_c\<^sub>1: "\<turnstile> (c\<^sub>1, Fault) \<rightarrow>\<^sup>* (Skip, Fault)" by fact
+  have steps_c\<^sub>2: "\<turnstile> (c\<^sub>2, Fault) \<rightarrow>\<^sup>* (Skip, Fault)" by fact
+  from SeqSteps [OF steps_c\<^sub>1 refl refl]
+  have "\<turnstile> (Seq c\<^sub>1 c\<^sub>2, Fault) \<rightarrow>\<^sup>* (Seq Skip c\<^sub>2, Fault)".
+  also
+  have "\<turnstile> (Seq Skip c\<^sub>2, Fault) \<rightarrow> (c\<^sub>2, Fault)" by (rule SeqSkip)
+  also note steps_c\<^sub>2
+  finally show ?case by simp
+qed (fastforce intro: step.intros)+
+
+lemma step_Fault_prop:
+  assumes step: "\<turnstile> (c, s) \<rightarrow> (c', s')"
+  shows "s=Fault  \<Longrightarrow> s'=Fault"
+  using step step_Fault  by blast 
+
+lemma steps_Fault_prop:
+  assumes step: "\<turnstile> (c, s) \<rightarrow>\<^sup>* (c', s')"
+  shows "s=Fault  \<Longrightarrow> s'=Fault "
+  using step
+proof (induct rule: converse_rtranclp_induct2 [case_names Refl Trans])
+  case Refl thus ?case by simp
+next
+  case (Trans c s c'' s'')
+  thus ?case
+    by (auto intro: step_Fault)
+qed
+
+(* ************************************************************************ *)
+subsection \<open>Equivalence between Small-Step and Big-Step Semantics\<close>
+(* ************************************************************************ *)
+
+theorem exec_impl_steps:
+  assumes exec: "\<turnstile>\<langle>c,s\<rangle> \<Rightarrow> t"
+  shows "\<exists>c' t'. \<turnstile>(c,s) \<rightarrow>\<^sup>* (c',t') \<and> c'=Skip \<and> t'=t"
+using exec
+proof (induct) 
+  case (CondTrue \<sigma> b c1 \<delta> \<Q> \<sigma>' c2)
+  then show ?case
+    by (meson converse_rtranclp_into_rtranclp step.CondTrue)
+next
+  case (CondFalse \<sigma> b c2 \<delta> \<Q> \<sigma>' c1)
+  then show ?case by (meson converse_rtranclp_into_rtranclp step.CondFalse)
+next
+  case (WhileTrue \<sigma> b c \<delta> \<Q> \<sigma>' \<sigma>'')
+  then show ?case 
+    by (meson SeqSkip SeqSteps converse_rtranclp_into_rtranclp rtranclp_trans step.WhileTrue) 
+next
+  case (WhileFalse \<sigma> b c \<delta> \<Q>)
+  then show ?case
+    by (meson r_into_rtranclp step.WhileFalse)
+next
+  case (Seq C1 \<sigma> \<sigma>' C2 \<sigma>'')
+  then show ?case
+    by (meson SeqSkip SeqSteps rtranclp.rtrancl_into_rtrancl rtranclp_trans) 
+next
+  case (Fault_Prop C)
+  then show ?case
+    using steps_Fault by blast 
+qed (auto simp add: r_into_rtranclp step.intros)
+
+corollary exec_impl_steps_Normal:
+  assumes exec: "\<turnstile>\<langle>c,s\<rangle> \<Rightarrow> Normal t"
+  shows "\<turnstile>(c,s) \<rightarrow>\<^sup>* (Skip, Normal t)"
+using exec_impl_steps [OF exec]
+by auto
+
+corollary exec_impl_steps_Fault:
+  assumes exec: "\<turnstile>\<langle>c,s\<rangle> \<Rightarrow> Fault"
+  shows "\<turnstile>(c,s) \<rightarrow>\<^sup>* (Skip, Fault)"
+using exec_impl_steps [OF exec]
+by auto
+
+(* lemma step_Fault_end:
+  assumes step: "\<turnstile> (c\<^sub>1, s) \<rightarrow> (c\<^sub>1', s')"
+  shows "s'=Fault \<Longrightarrow> s=Fault" sorry
+(* proof (induct rule: step_induct[OF step],auto) 
+  
+end *) *)
+
+
+lemma step_extend:
+  assumes step: "\<turnstile>(c,s) \<rightarrow> (c', s')"
+  shows "\<And>t. \<turnstile>\<langle>c',s'\<rangle> \<Rightarrow> t \<Longrightarrow> \<turnstile>\<langle>c,s\<rangle> \<Rightarrow> t"
+  using step
+proof (induct)
+  case (StackMod f \<delta> \<sigma> \<Q>)
+  then show ?case 
+    using QExec.StackMod QSemanticsBig.vars.QExec_Normal_elim_cases(2) vars_axioms by blast 
+next
+  case (QMod q \<sigma> \<Q> M \<Q>' \<delta>)
+  then show ?case
+    by (metis QExec.QMod QSemanticsBig.vars.QExec_Normal_elim_cases(2) vars_axioms) 
+next
+  case (QMod_F q \<sigma> \<Q> M \<delta>)
+  then show ?case
+    by (metis QExec.QMod_F exec_Fault_end) 
+next
+  case (Alloc q' \<Q> v \<sigma> \<vv>' q'_addr \<sigma>' q \<delta>)
+  then show ?case
+    by (smt (verit, best) QSemanticsBig.vars.QExec_Normal_elim_cases(2) vars.QExec.Alloc vars_axioms) 
+next
+  case (Alloc_F v \<sigma> q \<delta> \<Q>)
+  then show ?case
+    using QExec.Alloc_F exec_Fault_end by blast 
+next
+  case (CondTrue \<sigma> b c1 c2 \<delta> \<Q>)
+  then show ?case
+    using QExec.CondTrue by auto 
+next
+  case (CondFalse \<sigma> b c1 c2 \<delta> \<Q>)
+  then show ?case
+    using QExec.CondFalse by blast 
+next
+  case (WhileTrue \<sigma> b c \<delta> \<Q>)
+  then show ?case using QExec.WhileTrue  vars_axioms
+    by (meson QSemanticsBig.vars.QExec_Normal_elim_cases(5))
+    
+next
+  case (WhileFalse \<sigma> b c \<delta> \<Q>)
+  then show ?case
+    by (metis QExec.WhileFalse QSemanticsBig.vars.QExec_Normal_elim_cases(2) vars_axioms) 
+next
+  case (Seq C1 \<sigma> C1' \<sigma>' C2)
+  then show ?case
+    by (smt (verit, ccfv_threshold) QExec.Fault_Prop QExec.Seq QSemanticsBig.vars.QExec_elim_cases(5) XQState.exhaust step_Fault_prop vars_axioms)
+next
+  case (SeqSkip C2 \<sigma>)
+  then show ?case
+    by (metis QExec.Fault_Prop QExec.Seq Skip XQState.exhaust exec_Fault_end) 
+next
+  case (Dispose \<Q>' \<Q>'' \<Q> q i \<sigma> \<delta>)
+  then show ?case
+    by (metis QExec.Dispose QSemanticsBig.vars.QExec_Normal_elim_cases(2) vars_axioms) 
+next
+  case (Dispose_F \<Q> q i \<sigma> \<delta>)
+  then show ?case
+    using QExec.Dispose_F exec_Fault_end by blast 
+next
+  case (Measure addr1 \<Q> q \<sigma> k \<delta>k \<Q>' \<delta>' \<delta> \<sigma>' v)
+  then show ?case
+    by (metis (mono_tags, lifting) QSemanticsBig.vars.QExec_Normal_elim_cases(2) vars.QExec.Measure vars_axioms) 
+next
+  case (Measure_F q \<sigma> \<Q> v \<delta>)
+  then show ?case
+    using QExec.Measure_F exec_Fault_end by blast 
+next
+  case (Fault_Prop c)
+  then show ?case
+    using QExec.Fault_Prop exec_Fault_end by blast 
+qed
+
+
+theorem steps_Skip_impl_exec:
+  assumes steps: "\<turnstile>(c,s) \<rightarrow>\<^sup>* (Skip,t)"
+  shows "\<turnstile>\<langle>c,s\<rangle> \<Rightarrow> t"
+using steps
+proof (induct rule: converse_rtranclp_induct2 [case_names Refl Trans])
+  case Refl thus ?case
+    by (cases t) (auto intro: QExec.intros)
+next
+  case (Trans c s c' s')
+  have "\<turnstile> (c, s) \<rightarrow> (c', s')" and "\<turnstile> \<langle>c',s'\<rangle> \<Rightarrow> t" by fact+
+  thus ?case
+    by (rule step_extend)
+qed
+
+(*lemma not_stuck:"\<turnstile>\<langle>c,Normal (p, \<sigma>, Q)\<rangle> \<Rightarrow> Fault \<or> 
+                 (\<exists> p' \<sigma>' Q'. \<turnstile>\<langle>c,Normal (p, \<sigma>, Q)\<rangle> \<Rightarrow> Normal (p',\<sigma>',Q'))"
+proof(induct c arbitrary: p \<sigma> Q)
+  case Skip
+  then show ?case
+    using QExec.Skip by blast 
+next
+  case (SMod x)
+  then show ?case
+    by (meson QExec.StackMod) 
+next
+  case (QMod x1 x2a)
+  then show ?case
+    by (metis vars.QExec.intros(3) vars.QExec.intros(4) vars_axioms) 
+next
+  case (IF x1 c1 c2)
+  then show ?case
+    by (metis QExec.CondFalse QExec.CondTrue) 
+next
+  case (While x1 c)
+  then show ?case sorry
+next
+  case (Seq c1 c2)
+  then show ?case
+    using QExec.Fault_Prop QExec.Seq by blast 
+next
+  case (Measure x1 x2a)
+  then show ?case sorry
+next
+  case (Alloc x1 x2a)
+  then show ?case sorry
+next
+  case (Dispose x1 x2a)
+  then show ?case
+    by (metis vars.QExec.intros(12) vars.QExec.intros(13) vars_axioms) 
+qed
+*)
+fun while_unfold::"nat \<Rightarrow> ('v, 's) com \<Rightarrow> 's assn \<Rightarrow> 's XQState \<Rightarrow> bool"
+  where "while_unfold 0 c b s = (s = Fault \<or> (\<exists>p \<sigma> Q. s = Normal (p, \<sigma>, Q) \<and> \<sigma>\<notin>b))" 
+  | "while_unfold (Suc n) c b s = 
+       (\<exists>p \<sigma> Q s'. s = Normal (p, \<sigma>, Q) \<and> \<sigma>\<in>b \<and> \<turnstile>\<langle>c,Normal (p, \<sigma>, Q)\<rangle> \<Rightarrow> s' \<and> while_unfold n c b s')"
+
+inductive QExec\<^sub>n::"nat \<Rightarrow> ('v, 's) com \<Rightarrow> 's assn \<Rightarrow> 's XQState \<Rightarrow> 's XQState \<Rightarrow> bool"
+  where "(s = Normal (p,\<sigma>,Q) \<and> \<sigma>\<notin>b) \<or> s = Fault \<Longrightarrow>  QExec\<^sub>n 0 c b s s"
+        | "s = Normal (p, \<sigma>, Q)  \<Longrightarrow> \<sigma>\<in>b \<Longrightarrow> \<turnstile>\<langle>c,s\<rangle> \<Rightarrow> s' \<Longrightarrow> QExec\<^sub>n n c b s' s'' \<Longrightarrow> 
+         QExec\<^sub>n (Suc n) c b s s''" 
+
+lemma QExec_QExec_n_aux:
+  assumes a0:"\<turnstile>\<langle>v,s\<rangle> \<Rightarrow> s'"
+  shows "v = While b c \<Longrightarrow> s1 = s \<Longrightarrow> s1' = s' \<Longrightarrow> \<exists>n. QExec\<^sub>n n c b s1 s1'"
+  using a0 
+proof(induct arbitrary: s1 s1')
+  case (WhileTrue \<sigma> b c \<delta> \<Q> \<sigma>' \<sigma>'')
+  have "\<exists>n. QExec\<^sub>n n c b \<sigma>'  \<sigma>''"
+    using WhileTrue.hyps(5) WhileTrue.prems(1) by force
+  then show ?case
+    using QExec\<^sub>n.intros(2) WhileTrue.hyps(1) WhileTrue.hyps(2) WhileTrue.prems(1) WhileTrue.prems(2) WhileTrue.prems(3) by blast 
+next
+  case (WhileFalse \<sigma> b c \<delta> \<Q>)
+  then show ?case
+    using QExec\<^sub>n.intros(1) by blast 
+next
+  case (Fault_Prop C)
+  then show ?case
+    using QExec\<^sub>n.intros(1) by blast 
+qed(auto)
+
+
+lemma QExec_QExec_n: assumes a0:"\<turnstile>\<langle>While b c,s\<rangle> \<Rightarrow> s'" 
+  shows "\<exists>n. QExec\<^sub>n n c b s s'"
+  using QExec_QExec_n_aux[OF a0] by auto
+
+lemma QExec_n_QExec: 
+  assumes a0: "QExec\<^sub>n n c b s s'"
+  shows "\<turnstile>\<langle>While b c,s\<rangle> \<Rightarrow> s'"
+  using a0
+proof(induct n arbitrary: s s')
+  case 0
+  then have "s = s'"
+    using QExec\<^sub>n.cases by blast
+  { assume "s = Fault"
+    then have ?case
+      using QExec.Fault_Prop \<open>s = s'\<close> by presburger 
+  } 
+  moreover{
+    fix p \<sigma> Q
+    assume "s = Normal (p, \<sigma>, Q)"
+    then have ?case
+      by (metis "0" QExec.WhileFalse QExec\<^sub>n.simps calculation old.nat.distinct(2))
+  }
+  ultimately show ?case
+    by (metis "0" QExec\<^sub>n.simps) 
+next
+  case (Suc n)
+  then obtain s'' p \<sigma> Q where 
+   "s = Normal (p, \<sigma>, Q)" and  "\<sigma>\<in>b" and "\<turnstile>\<langle>c,s\<rangle> \<Rightarrow> s''" and "QExec\<^sub>n n c b s'' s'"
+    by (smt (verit, ccfv_SIG) QExec\<^sub>n.simps nat.inject old.nat.distinct(2))
+  then show ?case
+    using QExec.WhileTrue Suc.hyps by blast 
+qed
+
+theorem QExec_n_eq_QExec: 
+  shows "(\<exists>n. QExec\<^sub>n n c b s s') = \<turnstile>\<langle>While b c,s\<rangle> \<Rightarrow> s'"
+  using QExec_n_QExec QExec_QExec_n by auto
+
+
+end
 
 end
 
